generational/spec/GC.Gen.CheneyGraphReadiness.fst
@@ -4156,6 +4156,94 @@ let chunked_cheney_collect_then_major_gc_live_subgraph_from_pre_promote_nonblue_
     minor major fp roots alloc_fuel fresh major_roots cap mark_fuel
 #pop-options
 
+#push-options "--z3rlimit 5 --fuel 0 --ifuel 0 --split_queries always"
+let chunked_cheney_collect_then_major_gc_live_subgraph_from_pre_promote_raw_field_target_policy
+  (minor: minor_state) (major: MH.major_heap) (fp: U64.t)
+  (roots: seq U64.t) (alloc_fuel: nat) (fresh: MH.heap_chunk)
+  (major_roots: seq obj_addr)
+  (cap: nat{cap > 0})
+  (mark_fuel: nat)
+  : Lemma
+    (requires
+      minor_wf minor /\
+      alloc_fuel > 1 /\
+      GenInv.chunked_collection_heap_shape minor major fp alloc_fuel /\
+      SpecMajorAlloc.major_fl_chain_terminates major fp alloc_fuel = true /\
+      GenInv.chunked_chain_objects_blue major fp alloc_fuel /\
+      chunked_minor_preflight_value_policy minor major fp roots fresh /\
+      CInj.chunked_minor_major_fields_nonblue_non_infix_targets minor major /\
+      GenMajorGCBridge.chunked_major_raw_field_targets_in_major major /\
+      GenMajorGCBridge.chunked_major_field_targets_non_infix major /\
+      (SpecMajorAlloc.major_fl_head_wosize major fp <
+       PromotionDemand.minor_promotion_demand minor + 1 ==>
+       CInj.chunked_minor_fields_miss_chunk minor fresh) /\
+      (let r =
+       SpecMajorAlloc.ensure_major_head_capacity_spec
+       major fp alloc_fuel
+       (PromotionDemand.minor_promotion_demand minor + 1)
+       fresh in
+       let collect =
+       ChunkedCheney.chunked_cheney_collect_spec
+       minor r.capacity_major_out r.capacity_fp_out roots
+       r.capacity_fuel_out in
+       GenInv.chunked_collection_heap_shape
+       collect.cmc_minor collect.cmc_major collect.cmc_fp
+       r.capacity_fuel_out /\
+       GenMajorGCBridge.chunked_major_roots_nonblue
+       collect.cmc_major major_roots /\
+       GenMajorGCBridge.chunked_major_edge_gen_field_witness
+       collect.cmc_major /\
+       GenMajorGCBridge.chunked_major_field_targets_non_infix
+       collect.cmc_major /\
+       CheneyPres.chunked_cheney_promote_split_ready
+       minor r.capacity_major_out r.capacity_fp_out roots
+       r.capacity_fuel_out /\
+       Seq.length (MH.major_objects collect.cmc_major) <= cap /\
+       mark_fuel > 0 /\
+       mark_fuel >= Seq.length (MH.major_objects collect.cmc_major)))
+    (ensures
+      chunked_cheney_collect_after_minor_promotion_head_preflight_post
+       minor major fp roots alloc_fuel fresh /\
+      (let r =
+       SpecMajorAlloc.ensure_major_head_capacity_spec
+       major fp alloc_fuel
+       (PromotionDemand.minor_promotion_demand minor + 1)
+       fresh in
+       let collect =
+       ChunkedCheney.chunked_cheney_collect_spec
+       minor r.capacity_major_out r.capacity_fp_out roots
+       r.capacity_fuel_out in
+       let (major_final, fp_final) =
+       ChunkedMajorGC.chunked_major_gc_bounded
+       (ChunkedMajorGCRoots.chunked_gray_roots
+         collect.cmc_major major_roots)
+       cap mark_fuel in
+       ChunkedMajorGCGraph.chunked_major_live_subgraph_preserved
+       collect.cmc_major major_final
+       (ChunkedMajorGCCorr.chunked_major_initial_reachable_live
+        collect.cmc_major major_roots)))
+  =
+  assert (chunked_preflight_base_policy minor major roots);
+  assert (chunked_major_chunks_above_zero_addr major);
+  chunked_major_chunks_above_zero_addr_objects_are_pointer_fields major;
+  let prove_pointer_field (target: obj_addr)
+    : Lemma
+        (requires Seq.mem target (MH.major_objects major))
+        (ensures Fields.is_pointer_field target)
+    =
+    chunked_major_objects_are_pointer_fields_elim major target
+  in
+  Classical.forall_intro
+    (Classical.move_requires prove_pointer_field);
+  GenInv.chunked_collection_heap_shape_elim minor major fp alloc_fuel;
+  assert (GenInv.chunked_major_alloc_shape major fp alloc_fuel);
+  GenInv.chunked_major_alloc_shape_elim major fp alloc_fuel;
+  CInj.chunked_nonblue_scanned_raw_targets_in_major_from_major_raw_field_targets
+    major;
+  chunked_cheney_collect_then_major_gc_live_subgraph_from_pre_promote_nonblue_static_raw_target_policy
+    minor major fp roots alloc_fuel fresh major_roots cap mark_fuel
+#pop-options
+
 let chunked_cheney_collect_then_major_gc_live_subgraph_from_raw_field_target_policy
   (minor: minor_state) (major: MH.major_heap) (fp: U64.t)
   (roots: seq U64.t) (alloc_fuel: nat) (fresh: MH.heap_chunk)
